pulse/lib/pulse/lib/Pulse.Lib.HigherArray.Core.fsti
@@ -1,5 +1,5 @@
 (*
-   Copyright 2023 Microsoft Research
+   Copyright 2025 Microsoft Research
 
    Licensed under the Apache License, Version 2.0 (the "License");
    you may not use this file except in compliance with the License.
@@ -14,7 +14,7 @@
    limitations under the License.
 *)
 
-module Pulse.Lib.Array.Core
+module Pulse.Lib.HigherArray.Core
 #lang-pulse
 open FStar.Tactics.V2
 open Pulse.Lib.Core
@@ -23,27 +23,22 @@ open Pulse.Class.PtsTo
 open PulseCore.FractionalPermission
 open FStar.Ghost
 module SZ = FStar.SizeT
-module Seq = FStar.Seq
 
 [@@erasable] val base_t : Type0
 
-inline_for_extraction
-val array ([@@@strictly_positive] a:Type u#0) : Type u#0
+val array ([@@@unused] a:Type u#1) : Type u#0
 
-val length (#a:Type u#0) (x:array a) : Ghost nat (requires True) (ensures SZ.fits)
+val length (#a:Type) (x:array a) : Ghost nat (requires True) (ensures SZ.fits)
 val base_of #t (a: array t) : base_t
 val offset_of #t (a: array t) : GTot nat
 
 type elseq (a:Type) (l:SZ.t) = s:erased (Seq.seq a) { Seq.length s == SZ.v l }
 
-inline_for_extraction
 type larray t (n:nat) = a:array t { length a == n }
 
-val is_full_array (#a:Type u#0) (x:array a) : prop
+val is_full_array (#a:Type) (x:array a) : prop
 
-inline_for_extraction
 val null #a : array a
-inline_for_extraction
 val is_null #a (r: array a) : b:bool {b <==> r == null #a}
 
 val pts_to_mask #t ([@@@mkey] a: array t) (#[full_default()] f: perm) (v: erased (Seq.seq t)) (mask: nat -> prop) : slprop
@@ -56,6 +51,12 @@ ghost
 fn pts_to_mask_len #t (a:array t) (#p:perm) (#x:Seq.seq t) #mask
   preserves pts_to_mask a #p x mask
   ensures pure (length a == Seq.length x)
+
+ghost
+fn pts_to_mask_perm_bound #t (arr: array t) #p (#s:Seq.seq t) #mask
+  preserves pts_to_mask arr #p s mask
+  requires pure (exists (i: nat). i < Seq.length s /\ mask i)
+  ensures pure (p <=. 1.0R)
 
 ghost
 fn pts_to_mask_not_null #a #p (r:array a) (#v:Seq.seq a) #mask
@@ -80,6 +81,16 @@ ghost fn mask_ext #t (arr: array t) #f #v #mask v' (mask': nat -> prop)
     (forall (i: nat). mask i /\ i < Seq.length v ==> Seq.index v i == Seq.index v' i))
   ensures pts_to_mask arr #f v' mask'
 
+fn mask_alloc #elt (x: elt) (n: SZ.t)
+  returns a: array elt
+  ensures pts_to_mask a (Seq.create (SZ.v n) x) (fun _ -> True)
+  ensures pure (length a == SZ.v n /\ is_full_array a)
+
+fn mask_free #elt (a: array elt) (#s: Ghost.erased (Seq.seq elt)) #mask
+  requires pts_to_mask a s mask
+  requires pure (forall i. mask i)
+  requires pure (is_full_array a)
+
 ghost
 fn mask_share #a (arr:array a) (#s: Seq.seq a) #p #mask
   requires pts_to_mask arr #p s mask
@@ -97,7 +108,8 @@ ghost fn mask_gather #t (arr: array t) #p1 #p2 #s1 #s2 #mask1 #mask2
 
 // We need to give names to these combinators, otherwise unfold can't
 // distinguish them when we have multiple pts_to_mask resources.
-include Pulse.Lib.HigherArray {mask_isect, mask_diff}
+unfold let mask_isect (mask pred: nat -> prop) : nat -> prop = fun i -> mask i /\ pred i
+unfold let mask_diff (mask pred: nat -> prop) : nat -> prop = fun i -> mask i /\ ~(pred i)
 
 ghost fn split_mask #t (arr: array t) #f #v #mask (pred: nat -> prop)
   requires pts_to_mask arr #f v mask
@@ -132,14 +144,12 @@ fn pts_to_mask_injective_eq #a #p0 #p1 #s0 #s1 #mask0 #mask1 (arr:array a)
     (forall (i: nat). i < Seq.length s0 /\ mask0 i /\ mask1 i ==>
       Seq.index s0 i == Seq.index s1 i))
 
-inline_for_extraction
 fn mask_read #t (a: array t) (i: SZ.t) #p (#s: erased (Seq.seq t) { SZ.v i < Seq.length s }) #mask
   preserves pts_to_mask a #p s mask
   requires pure (mask (SZ.v i))
   returns res: t
   ensures pure (res == Seq.index s (SZ.v i))
 
-inline_for_extraction
 fn mask_write #t (a: array t) (i: SZ.t) (v: t) (#s: erased (Seq.seq t) { SZ.v i < Seq.length s }) #mask
   requires pts_to_mask a s mask
   requires pure (mask (SZ.v i))
@@ -147,9 +157,13 @@ fn mask_write #t (a: array t) (i: SZ.t) (v: t) (#s: erased (Seq.seq t) { SZ.v i 
 
 val gsub #t (arr: array t) (i: nat) (j: nat { i <= j /\ j <= length arr }) : GTot (array t)
 
+val length_gsub #t arr i j : Lemma (length (gsub #t arr i j) == j - i) [SMTPat (length (gsub arr i j))]
+val offset_of_gsub #t arr i j : Lemma (offset_of (gsub #t arr i j) == offset_of arr + i) [SMTPat (offset_of (gsub arr i j))]
+val base_of_gsub #t arr i j : Lemma (base_of (gsub #t arr i j) == base_of arr) [SMTPat (base_of (gsub arr i j))]
+
 ghost fn gsub_intro #t (arr: array t) #f #mask (i j: nat) (#v: erased (Seq.seq t) { i <= j /\ j <= Seq.length v })
   requires pts_to_mask arr #f v mask
-  requires pure (forall (k: nat). mask k ==> i <= k /\ k < j)
+  requires pure (forall (k: nat). mask k /\ k < Seq.length v ==> i <= k /\ k < j)
   returns _: squash (length arr == Seq.length v)
   ensures pts_to_mask (gsub arr i j) #f (Seq.slice v i j) (fun k -> mask (k + i))
 
@@ -157,11 +171,10 @@ ghost fn gsub_elim #t (arr: array t) #f (#mask: nat->prop) (i j: nat)
     (#v: erased (Seq.seq t) { i <= j /\ j <= length arr })
   requires pts_to_mask (gsub arr i j) #f v mask
   returns _: squash (j - i == Seq.length v)
-  ensures exists* v'.
+  ensures exists* (v': Seq.seq t).
     pts_to_mask arr #f v' (fun k -> i <= k /\ k < j /\ mask (k - i)) **
     pure (Seq.length v' == length arr /\ (forall (k:nat). k < j - i ==> Seq.index v k == Seq.index v' (k + i)))
 
-inline_for_extraction
 unobservable
 fn sub #t (arr: array t) #f #mask (i: SZ.t) (j: SZ.t)
     (#v: erased (Seq.seq t) { SZ.v i <= SZ.v j /\ SZ.v j <= Seq.length (reveal v) })
@@ -180,230 +193,3 @@ ghost fn return_sub #t (arr: array t) #f (#v #vsub: erased (Seq.seq t)) #mask #m
     ** pure (Seq.length v == Seq.length v' /\ i + Seq.length vsub == j /\ j <= Seq.length v /\
       (forall (k: nat). k < Seq.length v' ==>
       Seq.index v' k == (if i <= k && k < j then Seq.index vsub (k - i) else Seq.index v k)))
-
-val pts_to (#a:Type u#0) ([@@@mkey]x:array a) (#[exact (`1.0R)] p:perm) (s: Seq.seq a) : slprop
-
-[@@pulse_unfold]
-instance has_pts_to_array (a:Type u#0) : has_pts_to (array a) (Seq.seq a) = {
-  pts_to = pts_to;
-}
-[@@pulse_unfold]
-instance has_pts_to_larray (a:Type u#0) (n : nat) : has_pts_to (larray a n) (Seq.seq a) = {
-  pts_to = pts_to;
-}
-
-ghost fn to_mask #t (arr: array t) #f #v
-  requires arr |-> Frac f v
-  ensures pts_to_mask arr #f v (fun _ -> True)
-
-ghost fn from_mask #t (arr: array t) #f #v #mask
-  requires pts_to_mask arr #f v mask
-  requires pure (forall i. mask i)
-  ensures arr |-> Frac f v
-
-val pts_to_timeless (#a:Type) (x:array a) (p:perm) (s:Seq.seq a)
-  : Lemma (timeless (pts_to x #p s))
-          [SMTPat (timeless (pts_to x #p s))]
-
-ghost
-fn pts_to_len (#t:Type0) (a:array t) (#p:perm) (#x:Seq.seq t)
-  requires pts_to a #p x
-  ensures  pts_to a #p x ** pure (length a == Seq.length x)
-
-[@@deprecated "Array.Core.alloc is meant to be generated by the Pulse elaborator, not called directly; use Vec.alloc instead"]
-inline_for_extraction
-fn alloc (#elt: Type) (x: elt) (n: SZ.t)
-  requires emp
-  returns  a : array elt
-  ensures  pts_to a (Seq.create (SZ.v n) x) **
-           pure (length a == SZ.v n /\ is_full_array a)
-
-(* Written x.(i) *)
-inline_for_extraction
-fn op_Array_Access
-  (#t: Type) (a: array t) (i: SZ.t)
-  (#p: perm) (#s: erased (Seq.seq t){SZ.v i < Seq.length s})
-  preserves pts_to a #p s
-  returns  res : t
-  ensures  rewrites_to res (Seq.index s (SZ.v i))
-
-(* Written a.(i) <- v *)
-inline_for_extraction
-fn op_Array_Assignment
-        (#t: Type)
-        (a: array t)
-        (i: SZ.t)
-        (v: t)
-        (#s: erased (Seq.seq t) {SZ.v i < Seq.length s})
-  requires pts_to a s
-  ensures  pts_to a (Seq.upd s (SZ.v i) v)
-
-[@@deprecated "Array.Core.free is not meant to be called directly; use Vec.free instead"]
-inline_for_extraction
-fn free (#elt: Type) (a: array elt) (#s: erased (Seq.seq elt))
-  requires pts_to a s ** pure (is_full_array a)
-  ensures emp
-
-ghost
-fn share
-  (#a:Type)
-  (arr:array a)
-  (#s:erased (Seq.seq a))
-  (#p:perm)
-  requires pts_to arr #p s
-  ensures  pts_to arr #(p /. 2.0R) s ** pts_to arr #(p /. 2.0R) s
-
-[@@allow_ambiguous]
-ghost
-fn gather
-  (#a:Type)
-  (arr:array a)
-  (#s0 #s1:erased (Seq.seq a))
-  (#p0 #p1:perm)
-  requires pts_to arr #p0 s0 ** pts_to arr #p1 s1
-  ensures  pts_to arr #(p0 +. p1) s0 ** pure (s0 == s1)
-
-val pts_to_range
-  (#a:Type u#0)
-  ([@@@mkey] x:array a)
-  ([@@@mkey] i : nat)
-  (j : nat)
-  (* ^NOTE: only using the start as matching key. *)
-  (#[exact (`1.0R)] p:perm)
-  (s: Seq.seq a) : slprop
-
-val pts_to_range_timeless (#a:Type) (x:array a) (i j : nat) (p:perm) (s:Seq.seq a)
-  : Lemma (timeless (pts_to_range x i j #p s))
-          [SMTPat (timeless (pts_to_range x i j #p s))]
-
-let is_subarray #elt (a: array elt) (i j: nat) (b: array elt) : prop =
-  base_of b == base_of a /\
-  offset_of b == offset_of a + i /\
-  i + length b == j /\
-  j <= length a
-
-ghost
-fn pts_to_range_prop
-  (#elt: Type0) (a: array elt) (#i #j: nat)
-  (#p: perm)
-  (#s: Seq.seq elt)
-  requires pts_to_range a i j #p s
-  ensures  pts_to_range a i j #p s
-           ** pure ( (i <= j /\ j <= length a /\ Seq.length s == j - i))
-
-ghost
-fn pts_to_range_intro
-  (#elt: Type0) (a: array elt)
-  (p: perm)
-  (s: Seq.seq elt)
-  requires pts_to a #p s
-  ensures  pts_to_range a 0 (length a) #p s
-
-ghost
-fn pts_to_range_elim
-  (#elt: Type0) (a: array elt)
-  (p: perm)
-  (s: Seq.seq elt)
-  requires pts_to_range a 0 (length a) #p s
-  ensures  pts_to a #p s
-
-ghost
-fn pts_to_range_split
-  (#elt: Type0)
-  (a: array elt)
-  (i m j: nat)
-  (#p: perm)
-  (#s: Seq.seq elt)
- requires pts_to_range a i j #p s ** pure (i <= m /\ m <= j)
- ensures
-   exists* s1 s2.
-     pts_to_range a i m #p s1 **
-     pts_to_range a m j #p s2 **
-     pure (
-       i <= m /\ m <= j /\ j <= length a /\
-       eq2 #int (Seq.length s) (j - i) /\
-       s1 == Seq.slice s 0 (m - i) /\
-       s2 == Seq.slice s (m - i) (Seq.length s) /\
-       s == Seq.append s1 s2
-     )
-
-ghost
-fn pts_to_range_join
-  (#elt: Type0)
-  (a: array elt)
-  (i m j: nat)
-  (#p: perm)
-  (#s1 #s2: Seq.seq elt)
-  requires pts_to_range a i m #p s1 ** pts_to_range a m j #p s2
-  ensures  pts_to_range a i j #p (s1 `Seq.append` s2)
-
-inline_for_extraction
-fn pts_to_range_index
-  (#t: Type)
-  (a: array t)
-  (i: SZ.t)
-  (#l: erased nat{l <= SZ.v i})
-  (#r: erased nat{SZ.v i < r})
-  (#s: erased (Seq.seq t))
-  (#p: perm)
-  requires pts_to_range a l r #p s
-  returns  res : t
-  ensures pts_to_range a l r #p s **
-          pure (eq2 #int (Seq.length s) (r - l) /\
-                res == Seq.index s (SZ.v i - l))
-
-inline_for_extraction
-fn pts_to_range_upd
-  (#t: Type)
-  (a: array t)
-  (i: SZ.t)
-  (v: t)
-  (#l: erased nat{l <= SZ.v i})
-  (#r: erased nat{SZ.v i < r})
-  (#s0: erased (Seq.seq t))
-  requires pts_to_range a l r s0
-  ensures
-    exists* s.
-      pts_to_range a l r s **
-      pure(
-        eq2 #int (Seq.length s0) (r - l) /\
-        s == Seq.upd s0 (SZ.v i - l) v
-      )
-
-ghost
-fn pts_to_range_share
-  (#a:Type)
-  (arr:array a)
-  (#l #r: nat)
-  (#s:Seq.seq a)
-  (#p:perm)
-  requires pts_to_range arr l r #p s
-  ensures  pts_to_range arr l r #(p /. 2.0R) s **
-           pts_to_range arr l r #(p /. 2.0R) s
-
-[@@allow_ambiguous]
-ghost
-fn pts_to_range_gather
-  (#a:Type)
-  (arr:array a)
-  (#l #r: nat)
-  (#s0 #s1: Seq.seq a)
-  (#p0 #p1:perm)
-  requires pts_to_range arr l r #p0 s0 ** pts_to_range arr l r #p1 s1
-  ensures  pts_to_range arr l r #(p0 +. p1) s0 **
-           pure (s0 == s1)
-
-(* Called by elaboration, not to be used directly. *)
-val with_local
-  (#a:Type0)
-  (init:a)
-  (len:SZ.t)
-  (#pre:slprop)
-  (ret_t:Type)
-  (#post:ret_t -> slprop)
-  (body:(arr:array a) -> stt ret_t (pre **
-                                    (pts_to arr (Seq.create (SZ.v len) init) **
-                                     (pure (is_full_array arr) **
-                                      pure (length arr == SZ.v len))))
-                                   (fun r -> post r ** (exists* v. pts_to arr v)))
-  : stt ret_t pre post
