pulse/lib/common/Pulse.Lib.Raise.fsti
@@ -1,0 +1,51 @@
+(*
+   Copyright 2025 Microsoft Research
+
+   Licensed under the Apache License, Version 2.0 (the "License");
+   you may not use this file except in compliance with the License.
+   You may obtain a copy of the License at
+
+       http://www.apache.org/licenses/LICENSE-2.0
+
+   Unless required by applicable law or agreed to in writing, software
+   distributed under the License is distributed on an "AS IS" BASIS,
+   WITHOUT WARRANTIES OR CONDITIONS OF ANY KIND, either express or implied.
+   See the License for the specific language governing permissions and
+   limitations under the License.
+*)
+module Pulse.Lib.Raise
+open FStar.ExtractAs
+
+// This is a re-export of FStar.Universe with better extraction rules and SMT patterns
+
+(** [raise_t a] is an isomorphic copy of [a] (living in universe 'ua) in universe [max 'ua 'ub] **)
+inline_for_extraction [@@extract_as (`(fun (t: Type u#a) -> t))]
+val raise_t ([@@@strictly_positive] t : Type u#a) : Type u#(max a b)
+
+(** [raise_val x] injects a value [x] of type [a] to [raise_t a] **)
+inline_for_extraction [@@extract_as (`(fun (#a: Type u#a) (x: a) -> x))]
+val raise_val : #a:Type u#a -> x:a -> raise_t u#a u#b a
+
+(** [downgrade_val x] projects a value [x] of type [raise_t a] to [a] **)
+inline_for_extraction [@@extract_as (`(fun (#a: Type u#a) (x: a) -> x))]
+val downgrade_val : #a:Type u#a -> x:raise_t u#a u#b a -> a
+
+val downgrade_val_raise_val
+  (#a: Type u#a)
+  (x: a)
+: Lemma
+  (downgrade_val u#a u#b (raise_val x) == x)
+  [SMTPat (raise_val x)]
+
+val raise_val_downgrade_val
+  (#a: Type u#a)
+  (x: raise_t u#a u#b a)
+: Lemma
+  (raise_val (downgrade_val x) == x)
+  [SMTPat (downgrade_val x)]
+
+let lift_dom #a #b (q:a -> b) : raise_t a -> b =
+  fun v -> q (downgrade_val v)
+
+let lift_codom #a #b (q:a -> b) : a -> raise_t b =
+  fun v -> raise_val (q v)
