pulse/lib/core/PulseCore.MemoryAlt.fsti
@@ -18,7 +18,7 @@ module PulseCore.MemoryAlt
 open FStar.Ghost
 open FStar.PCM
 module PST = PulseCore.HoareStateMonad
-module U = FStar.Universe
+module U = Pulse.Lib.Raise
 module CM = FStar.Algebra.CommMonoid
 module B = PulseCore.BaseHeapSig
 
