pulse/lib/pulse/lib/Pulse.Lib.HigherArray.PtsTo.fst
@@ -1,0 +1,196 @@
+(*
+   Copyright 2025 Microsoft Research
+
+   Licensed under the Apache License, Version 2.0 (the "License");
+   you may not use this file except in compliance with the License.
+   You may obtain a copy of the License at
+
+       http://www.apache.org/licenses/LICENSE-2.0
+
+   Unless required by applicable law or agreed to in writing, software
+   distributed under the License is distributed on an "AS IS" BASIS,
+   WITHOUT WARRANTIES OR CONDITIONS OF ANY KIND, either express or implied.
+   See the License for the specific language governing permissions and
+   limitations under the License.
+*)
+
+module Pulse.Lib.HigherArray.PtsTo
+#lang-pulse
+open Pulse.Main
+open FStar.Tactics.V2
+open Pulse.Lib.Core
+open PulseCore.FractionalPermission
+open FStar.Ghost
+module SZ = FStar.SizeT
+module Seq = FStar.Seq
+open Pulse.Lib.WithPure
+
+let pts_to (#elt: Type u#1) (a: array elt) (#p: perm) (s: Seq.seq elt) : Tot slprop =
+  pts_to_mask a #p s fun i -> True
+
+ghost fn to_mask #t (arr: array t) #f #v
+  requires arr |-> Frac f v
+  ensures pts_to_mask arr #f v (fun _ -> True)
+{
+  unfold pts_to arr #f v;
+}
+
+ghost fn from_mask #t (arr: array t) #f #v #mask
+  requires pts_to_mask arr #f v mask
+  requires pure (forall (i: nat). i < Seq.length v ==> mask i)
+  ensures arr |-> Frac f v
+{
+  mask_mext arr (fun _ -> True);
+  fold pts_to arr #f v;
+}
+
+let pts_to_timeless _ _ _ = ()
+
+ghost
+fn pts_to_len
+  (#elt: Type u#1)
+  (a:array elt)
+  (#p:perm)
+  (#x:Seq.seq elt)
+  requires pts_to a #p x
+  ensures pts_to a #p x ** pure (length a == Seq.length x)
+{
+  unfold pts_to a #p x;
+  pts_to_mask_len a;
+  fold pts_to a #p x;
+}
+
+ghost
+fn pts_to_not_null (#a:_) (#p:_) (r:array a) (#v:Seq.seq a)
+  preserves r |-> Frac p v
+  ensures  pure (not (is_null #a r))
+{
+  unfold pts_to r #p v;
+  pts_to_mask_not_null _;
+  fold pts_to r #p v;
+}
+
+inline_for_extraction
+fn alloc
+    (#elt: Type u#1)
+    (x: elt)
+    (n: SZ.t)
+  returns a:array elt
+ensures 
+  pts_to a (Seq.create (SZ.v n) x) **
+  pure (length a == SZ.v n /\ is_full_array a)
+{
+  let a = mask_alloc x n;
+  fold pts_to a (Seq.create (SZ.v n) x);
+  a
+}
+
+inline_for_extraction
+fn read
+    (#t: Type)
+    (a: array t)
+    (i: SZ.t)
+    (#p: perm)
+    (#s: Ghost.erased (Seq.seq t){SZ.v i < Seq.length s})
+  preserves pts_to a #p s
+  returns res:t
+  ensures pure (res == Seq.index s (SZ.v i))
+{
+  unfold pts_to a #p s;
+  let res = mask_read a i;
+  fold pts_to a #p s;
+  res
+}
+
+let op_Array_Access = read
+
+inline_for_extraction
+fn write
+    (#t: Type)
+    (a: array t)
+    (i: SZ.t)
+    (v: t)
+    (#s: Ghost.erased (Seq.seq t) {SZ.v i < Seq.length s})
+  requires pts_to a s
+  ensures pts_to a (Seq.upd s (SZ.v i) v)
+{
+  unfold pts_to a #1.0R s;
+  mask_write a i v;
+  fold pts_to a #1.0R (Seq.upd s (SZ.v i) v);
+}
+
+let op_Array_Assignment = write
+
+fn free
+    (#elt: Type)
+    (a: array elt)
+    (#s: Ghost.erased (Seq.seq elt))
+  requires pts_to a s
+  requires pure (is_full_array a)
+{
+  unfold pts_to a s;
+  mask_free a;
+}
+
+ghost
+fn share
+  (#elt:Type)
+  (arr:array elt)
+  (#s:Ghost.erased (Seq.seq elt))
+  (#p:perm)
+  requires pts_to arr #p s
+  ensures pts_to arr #(p /. 2.0R) s ** pts_to arr #(p /. 2.0R) s
+{
+  unfold pts_to arr #p s;
+  mask_share arr;
+  fold pts_to arr #(p /. 2.0R) s;
+  fold pts_to arr #(p /. 2.0R) s;
+}
+
+[@@allow_ambiguous]
+ghost
+fn gather
+  (#a:Type)
+  (arr:array a)
+  (#s0 #s1:Ghost.erased (Seq.seq a))
+  (#p0 #p1:perm)
+  requires pts_to arr #p0 s0 ** pts_to arr #p1 s1
+  ensures pts_to arr #(p0 +. p1) s0 ** pure (s0 == s1)
+{
+  unfold pts_to arr #p0 s0;
+  unfold pts_to arr #p1 s1;
+  mask_gather arr;
+  with v. assert pts_to_mask arr #(p0 +. p1) v (fun _ -> True);
+  assert pure (v `Seq.equal` s1 /\ v `Seq.equal` s0);
+  fold pts_to arr #(p0 +. p1) s0;
+}
+
+[@@allow_ambiguous]
+ghost
+fn pts_to_injective_eq
+    (#a:Type)
+    (#p0 #p1:perm)
+    (#s0 #s1:Seq.seq a)
+    (arr:array a)
+  preserves pts_to arr #p0 s0
+  preserves pts_to arr #p1 s1
+  ensures pure (s0 == s1)
+{
+  unfold pts_to arr #p0 s0;
+  unfold pts_to arr #p1 s1;
+  pts_to_mask_injective_eq arr;
+  assert pure (Seq.equal s0 s1);
+  fold pts_to arr #p0 s0;
+  fold pts_to arr #p1 s1;
+}
+
+ghost
+fn pts_to_perm_bound (#a:_) (#p:_) (arr: array a) (#s:Seq.seq a)
+  preserves pts_to arr #p s
+  requires pure (Seq.length s > 0)
+  ensures pure (p <=. 1.0R)
+{
+  unfold pts_to arr #p s;
+  pts_to_mask_perm_bound arr;
+  fold pts_to arr #p s;
+}
